michael_formal/Lift.thy
@@ -10,6 +10,9 @@ definition t1up :: "transition" where
         Updates = []
       \<rparr>"
 
+lemma updates_t1up [simp]:"Updates t1up = []"
+  by (simp add: t1up_def)
+
 definition t2up :: "transition" where
 "t2up \<equiv> \<lparr>
         Label = ''goUp'',
@@ -19,6 +22,12 @@ definition t2up :: "transition" where
         Updates = []
       \<rparr>"
 
+lemma updates_t2up [simp]:"Updates t2up = []"
+  by (simp add: t2up_def)
+
+lemma guard_t2up: "Guard t2up = [(gexp.Gt (V (I 1)) (L (Num 0)))]"
+  by (simp add: t2up_def)
+
 definition t3up :: "transition" where
 "t3up \<equiv> \<lparr>
         Label = ''goUp'',
@@ -27,6 +36,9 @@ definition t3up :: "transition" where
         Outputs = [(L (Num 0))],
         Updates = []
       \<rparr>"
+
+lemma updates_t3up [simp]:"Updates t3up = []"
+  by (simp add: t3up_def)
 
 definition t1down :: "transition" where
 "t1down \<equiv> \<lparr>
@@ -75,27 +87,86 @@ definition closeDoors :: transition where
 
 lemmas transitions = t1up_def t2up_def t3up_def t1down_def t2down_def t3down_def openDoors_def closeDoors_def
 
-definition lift :: "efsm" where
-"lift \<equiv> \<lparr> S = [1,2,3,4],
-          s0 = 1,
+datatype statename = q1 | q2 | q3 | q4
+
+definition lift :: "statename efsm" where
+"lift \<equiv> \<lparr>
+          s0 = q1,
           T = \<lambda> (a,b) . 
-                   if (a,b) = (1,2) then [t1up]
-              else if (a,b) = (2,2) then [t2up]
-              else if (a,b) = (2,1) then [t3up]
-              else if (a,b) = (1,3) then [t1down]
-              else if (a,b) = (3,3) then [t2down]
-              else if (a,b) = (3,1) then [t3down]
-              else if (a,b) = (1,4) then [openDoors]
-              else if (a,b) = (4,1) then [closeDoors]
-              else []
+                   if (a,b) = (q1,q2) then {t1up}
+              else if (a,b) = (q2,q2) then {t2up}
+              else if (a,b) = (q2,q1) then {t3up}
+              else if (a,b) = (q1,q3) then {t1down}
+              else if (a,b) = (q3,q3) then {t2down}
+              else if (a,b) = (q3,q1) then {t3down}
+              else if (a,b) = (q1,q4) then {openDoors}
+              else if (a,b) = (q4,q1) then {closeDoors}
+              else {}
          \<rparr>"
 
+lemma label_goup_q2: "Label b = ''goUp'' \<Longrightarrow> b \<in> T lift (s0 lift, a) \<Longrightarrow> a = q2 \<and> b = t1up"
+  apply (simp add: lift_def)
+  apply (cases a)
+     apply simp
+    apply simp
+   apply (simp add: t1down_def)
+  by (simp add: openDoors_def)
+
+lemma possible_steps_q1_goup: "possible_steps lift (s0 lift) Map.empty ''goUp'' [Num 1] = {(q2, t1up)}"
+  apply (simp add: possible_steps_def)
+  apply safe
+       apply (simp add: label_goup_q2)
+      apply (simp add: label_goup_q2)
+  prefer 2
+  apply (simp add: lift_def)
+  by (simp_all add: t1up_def)
+
+lemma label_goup_q2_2: "Label b = ''goUp'' \<Longrightarrow> b \<in> T lift (q2, a) \<Longrightarrow> a = q2 \<or> a = q1"
+  apply (simp add: lift_def)
+  apply (cases a)
+  by simp_all
+
+lemma t2up_q2_q2:  "Label b = ''goUp'' \<Longrightarrow> b \<in> T lift (q2, q2) = (b = t2up)"
+  by (simp add: lift_def)
+
+lemma t3up_q2_q1: "Label b = ''goUp'' \<Longrightarrow> b \<in> T lift (q2, q1) = (b = t3up)"
+  by (simp add: lift_def)
+
+lemma possible_steps_q2_goup: "possible_steps lift q2 Map.empty ''goUp'' [Num 0] = {(q1, t3up)}"
+  apply (simp add: possible_steps_def)
+  apply safe
+       apply (case_tac "a=q1")
+        apply simp
+       apply (case_tac "a=q2")
+        apply (simp add: t2up_q2_q2 guard_t2up)
+  using label_goup_q2_2 apply blast
+      apply (case_tac "a=q1")
+       apply (simp add: t3up_q2_q1)
+      apply (case_tac "a=q2")
+       apply (simp add: t2up_q2_q2 guard_t2up)
+  using label_goup_q2_2 apply blast
+     prefer 2
+     apply (simp add: lift_def)
+  by (simp_all add: t3up_def)
+
+lemma label_open_q4: "Label b = ''open'' \<Longrightarrow> b \<in> T lift (q1, a) \<Longrightarrow> b = openDoors \<and> a = q4"
+  apply (simp add: lift_def)
+  apply (cases a)
+     apply simp
+    apply (simp add: t1up_def)
+   apply (simp add: t1down_def)
+  by simp
+
+lemma possible_steps_open_q1: "(possible_steps lift q1 Map.empty ''open'' []) = {(q4, openDoors)}"
+  apply (simp add: possible_steps_def)
+  apply safe
+       apply (simp add: label_open_q4)
+      apply (simp add: label_open_q4)
+  prefer 2
+  apply (simp add: lift_def)
+  by (simp_all add: openDoors_def)
+
 lemma "observe_trace lift (s0 lift) <> [(''goUp'', [Num 1]), (''goUp'', [Num 0]), (''open'', [])] = [[Num 1], [Num 0], [Num 1]]"
-  by (simp add: step_def lift_def transitions)
-
-lemma "observe_trace lift (s0 lift) <> [(''goDown'', [Num 1]), (''goDown'', [Num 0]), (''open'', [])] = [[Num 1], [Num 0], [Num 1]]"
-  by (simp add: step_def lift_def transitions)
-
-lemma "observe_trace lift (s0 lift) <> [(''open'', []), (''close'', []), (''open'', [])] = [[Num 1], [Num 0], [Num 1]]"
-  by (simp add: step_def lift_def transitions)
+  apply (simp add: possible_steps_q1_goup possible_steps_q2_goup possible_steps_open_q1 del: One_nat_def)
+  by (simp add: transitions)
 end
