michael_formal/valid_aux.thy
@@ -6,22 +6,27 @@ abbreviation "reg_of t \<equiv> (if t = [] then <> else snd (snd (last t)))"
 abbreviation "state_of e t \<equiv> (if t = [] then s0 e else fst (last t))"
 
 lemma valid_trace_non_empty_observe: "valid_trace e (a#list) \<Longrightarrow> [] \<noteq> observe_all e (s0 e) <> (a # list)"
-  apply(simp only:observe_all.simps(2))
-  by auto
+  by fastforce
 
 lemma nonempty: "valid_trace e t \<and> t \<noteq> [] \<longrightarrow> observe_all e (s0 e) <> t \<noteq> []"
   by auto
 
-lemma valid_trace_head_not_none:  "valid_trace efsm [a] \<Longrightarrow> ( step efsm (s0 efsm) <> (fst a) (snd a) \<noteq> None)"
-  apply simp
-  apply(cases  "(step efsm (s0 efsm) <> (fst a) (snd a)) = None")
-  by(simp_all)
+lemma first_none_invalid: "step efsm (s0 efsm) <> (fst a) (snd a) = None \<Longrightarrow> \<not> valid_trace efsm [a]"
+  apply (cases "is_singleton (possible_steps efsm (s0 efsm) Map.empty (fst a) (snd a))")
+   apply simp
+  by simp
+
+lemma valid_trace_head_not_none:  "valid_trace efsm [a] \<Longrightarrow> (step efsm (s0 efsm) <> (fst a) (snd a) \<noteq> None)"
+  apply (rule ccontr)
+  using first_none_invalid by blast
 
 lemma valid_trace_cons: "valid_trace efsm (a#t) \<Longrightarrow> valid_trace efsm [a]"
   apply(simp)
-  apply(cases  "(step efsm (s0 efsm) <> (fst a) (snd a)) = None")
-  apply(simp)
-  by auto
+  apply (cases "is_singleton (possible_steps efsm (s0 efsm) Map.empty (fst a) (snd a))")
+   apply (simp add: the_elem_def)
+   apply (cases "THE x. possible_steps efsm (s0 efsm) Map.empty (fst a) (snd a) = {x}")
+   apply simp
+  by simp
 
 lemma length_observe_all_restricted: "\<And>s r. length (observe_all e s r t) \<le> length t"
 proof (induction t) 
